proof/Ax.v
@@ -1,0 +1,27 @@
+Set Warnings "-notation-overridden,-parsing".
+From PLF Require Import Maps.
+From PLF Require Import Types.
+(* From PLF Require Import Smallstep. *)
+From PLF Require Import CoreLangSimp.
+From PLF Require Import NormalTypeSystemSimp.
+From Coq Require Import Logic.FunctionalExtensionality.
+From Coq Require Import Logic.ClassicalFacts.
+
+Import NormalTypeSystemSimp.
+
+Definition state_permute {A:Type}: forall (st: string -> option A) x y (a a': A),
+    (x |-> a; y |-> a'; st) = (y |-> a'; x |-> a; st).
+Admitted.
+
+Definition exists_not_free_var_in_tm: forall e, exists x, ~ x \FVtm e.
+Admitted.
+
+Lemma closed_term_has_no_free_var: forall e x T, empty \N- e \Tin T -> ~ x \FVtm e.
+Admitted.
+
+(* for vfix Axiom *)
+Definition const_order: constant -> constant -> Prop.
+Admitted.
+
+Lemma const_order_is_well_founded: well_founded const_order.
+Admitted.
