proof/WellFormedSimp.v
@@ -74,30 +74,81 @@ Qed.
 
 Global Hint Resolve ctx_inv_implies_type_closed_ctx: core.
 
+Lemma tmR_in_ctx_pre_weakening: forall nst Gamma1 Gamma2 (tau: overunderty),
+    ctx_inv nst (Gamma1 ++ Gamma2) ->
+    st_type_closed_in_ctx (state_to_tystate nst) Gamma2 tau ->
+    (forall e, tmR_in_ctx_aux nst Gamma2 tau e -> tmR_in_ctx_aux nst (Gamma1 ++ Gamma2) tau e).
+Proof with eauto.
+  intros.
+  induction Gamma1...
+  - destruct a.
+    rewrite <- app_comm_cons in H.
+    assert (type_ctx_no_dup (st\_ nst _/) ((s, o) :: Gamma1 ++ Gamma2))...
+    apply type_ctx_no_dup_implies_head_free in H2. apply l_find_right_most_none_neq_hd in H2. exfalso...
+Qed.
+
+Lemma tmR_in_ctx_post_weakening: forall nst Gamma1 Gamma2 (tau: overunderty),
+    ctx_inv nst (Gamma1 ++ Gamma2) ->
+    st_type_closed_in_ctx (st\_ nst _/) Gamma1 tau ->
+    (forall e, tmR_in_ctx_aux nst Gamma1 tau e -> tmR_in_ctx_aux nst (Gamma1 ++ Gamma2) tau e).
+Proof with eauto.
+  intros.
+  induction Gamma1... simpl. eapply tmR_in_ctx_pre_weakening in H1. rewrite app_nil_r in H1. apply H1. rewrite app_nil_r ...
+  auto.
+  - destruct a.
+    rewrite <- app_comm_cons in H.
+    assert (type_ctx_no_dup (st\_ nst _/) ((s, o) :: Gamma1 ++ Gamma2))...
+    apply type_ctx_no_dup_implies_head_free in H2. apply l_find_right_most_none_neq_hd in H2. exfalso...
+Qed.
+
 Lemma ctx_inv_implies_no_dup: forall st Gamma,
     ctx_inv st Gamma -> type_ctx_no_dup (st\_ st _/) Gamma.
-Admitted.
+Proof with eauto.
+  intros. destruct H...
+Qed.
 
 Global Hint Resolve ctx_inv_implies_no_dup: core.
 
 Definition state_tystate_same_none: forall nst x, nst x = None <-> (st\_ nst _/) x = None.
-Admitted.
+Proof with eauto.
+  intros.
+  split; intros... unfold state_to_tystate. rewrite H... unfold state_to_tystate in H. destruct (nst x)...
+  inversion H.
+Qed.
 
 Global Hint Rewrite state_tystate_same_none: core.
 
-Lemma ctx_inv_destruct_underbase: forall Gamma nst x T phi (e_x: constant),
-    ctx_inv nst ((x, Uty ([[v:T | phi]])) :: Gamma) ->
-    (forall v_x, tmR_aux nst ([[v: T | phi]]) v_x ->
-            ctx_inv (x |-> e_x; nst) Gamma).
+Lemma ctx_inv_destruct_underbase: forall Gamma st id T phi e_x (v_x_hat: constant),
+    ctx_inv st ((id, Uty ([[v:T | phi]])) :: Gamma) ->
+    tmR_aux st ([[v:T | phi]]) e_x ->
+    e_x -->* v_x_hat ->
+    ctx_inv (id |-> v_x_hat; st) Gamma.
 Proof with eauto.
-Admitted.
+  apply (rev_ind (fun Gamma => forall  st id T phi e_x (v_x_hat: constant),
+                      ctx_inv st ((id, Uty ([[v:T | phi]])) :: Gamma) ->
+                      tmR_aux st ([[v:T | phi]]) e_x ->
+                      e_x -->* v_x_hat ->
+                      ctx_inv (id |-> v_x_hat; st) Gamma)).
+  - intros  st id T phi e_x v_x_hat Hinv He_xD HE.
+    apply destruct_ctx_inv_one in Hinv. destruct Hinv as (Hclosed & Hnotbot).
+    assert (empty \N- e_x \Tin (T)) as He_xT... eapply tmR_has_type in He_xD...
+  - intros (a & tau_a) Gamma Hind st id T phi e_x v_x_hat Hinv He_xD HE.
+    assert (type_ctx_no_dup (st\_ st _/) ((id, Uty ([[v:T | phi]])) :: Gamma ++ ((a, tau_a)::nil)))...
+    apply type_ctx_no_dup_implies_head_free in H. apply l_find_right_most_none_neq_hd in H. exfalso...
+Qed.
 
-(*   apply (rev_ind (fun Gamma => forall nst x phi (e_x: constant), *)
-(*                       ctx_inv nst ((x, Uty ([[v: T | phi]])) :: Gamma) -> *)
-(*                       tmR_aux nst ([[v: T | phi]]) e_x -> *)
-(*                       ctx_inv (x |-> e_x; nst) Gamma)). *)
-(*   - intros nst x phi e_x Hinv He_xD. *)
-(*     apply destruct_ctx_inv_one in Hinv. destruct Hinv as (Hwf & Hclosed & Hnotbot). *)
+(* Lemma ctx_inv_destruct_underbase: forall Gamma st x T phi (e_x: constant), *)
+(*     ctx_inv st ((id, Uty ([[v:T | phi]])) :: Gamma) -> *)
+(*     tmR_aux st ([[v:T | phi]]) e_x -> *)
+(*     e_x -->* v_x_hat -> *)
+(*     ctx_inv (id |-> v_x_hat; st) Gamma. *)
+(* Proof with eauto. *)
+(*   apply (rev_ind (fun Gamma => forall nst x T phi (e_x: constant), *)
+(*                       ctx_inv nst ((x, Uty ([[v:T | phi]])) :: Gamma) -> *)
+(*                       (forall v_x, tmR_aux nst ([[v: T | phi]]) v_x -> *)
+(*                               ctx_inv (x |-> e_x; nst) Gamma))). *)
+(*   - intros nst x T phi e_x Hinv v_x He_xD. *)
+(*     apply destruct_ctx_inv_one in Hinv. destruct Hinv as (Hclosed & Hnotbot). *)
 (*     assert (empty \N- e_x \Tin (T)) as He_xT... eapply tmR_has_type in He_xD... *)
 (*   - intros (a & tau_a) Gamma Hind nst x phi e_x Hinv He_xD. *)
 (*     rewrite app_comm_cons in Hinv... apply destruct_ctx_inv in Hinv... destruct Hinv as (H1 & H2 & H3). *)
@@ -126,7 +177,12 @@ Lemma inv_ctx_preserve_denotation: forall nst Gamma tau e,
     ctx_inv nst Gamma ->
     tmR_aux nst tau e ->
     tmR_in_ctx_aux nst Gamma tau e.
-Admitted.
+Proof with eauto.
+  intros.
+  induction Gamma. constructor...
+  - destruct a. assert (type_ctx_no_dup (st\_ nst _/) ((s, o) :: Gamma))...
+    apply type_ctx_no_dup_implies_head_free in H1. apply l_find_right_most_none_neq_hd in H1. exfalso...
+Qed.
 
 (* Lemma inv_ctx_implies_construct_arrarr: forall nst x t1 t2 Gamma tau e, *)
 (*     ctx_inv nst ((x, Uty (t1 u--> t2)) :: Gamma) -> *)
@@ -136,7 +192,12 @@ Admitted.
 
 Lemma inv_ctx_implies_head: forall nst x tau_x Gamma,
     ctx_inv nst ((x, tau_x) :: Gamma) -> ctx_inv nst [(x, tau_x)].
-Admitted.
+Proof with eauto.
+  intros.
+  induction Gamma...
+  - destruct a. assert (type_ctx_no_dup (st\_ nst _/) ((x, tau_x) :: (s, o) :: Gamma))...
+    apply type_ctx_no_dup_implies_head_free in H0. apply l_find_right_most_none_neq_hd in H0. exfalso...
+Qed.
 
 Lemma ctx_inv_destruct_underarrarr: forall Gamma nst x t1 t2,
     ctx_inv nst ((x, Uty (t1 u--> t2)) :: Gamma) -> ctx_inv nst Gamma.
@@ -151,8 +212,8 @@ Proof with eauto.
     constructor...
     + constructor; auto. inversion Hnodup... eapply st_type_closed_in_ctx_destruct_arrar_front in Htau...
     + intros. eapply H3... constructor...
-      rewrite state_tystate_same_none...
-      assert (l_find_right_most Gamma x = None) as Hfindx...
+      (* rewrite state_tystate_same_none... *)
+      (* assert (l_find_right_most Gamma x = None) as Hfindx... *)
       intros e_x He_xD. assert (exists c0 : constant, e_x -->* c0) as He_xE... apply inv_ctx_implies_head in H1. apply destruct_ctx_inv_one in H1. destruct H1...
       destruct tau_a.
       { eapply step_preserve_ctx_denotation... apply eta_drop_lete_not_bot... }
@@ -162,12 +223,35 @@ Qed.
 Lemma ctx_inv_destruct_underoarr: forall Gamma nst x a T phia tau_b,
     ctx_inv nst ((x, Uty (a o: ({{v:T | phia}}) o--> tau_b)) :: Gamma) -> ctx_inv nst Gamma.
 Proof with eauto.
-Admitted.
+  apply (rev_ind (fun Gamma => forall nst x a T phia tau_b,
+                      ctx_inv nst ((x, Uty (a o: ({{v:T | phia}}) o--> tau_b)) :: Gamma) -> ctx_inv nst Gamma))...
+  - intros (a & tau_a) Gamma Hind nst x y T phiy tau_b Hinv.
+    assert (type_ctx_no_dup (st\_ nst _/) ((x, Uty (y o: {{v:T | phiy}} o--> tau_b)) :: Gamma <l> a :l: tau_a)) as Hnodup. apply ctx_inv_implies_no_dup in Hinv...
+    rewrite app_comm_cons in Hinv... apply destruct_ctx_inv in Hinv... destruct Hinv as (H1 & H2 & H3).
+    assert (ctx_inv nst Gamma) as Hinv...
+    apply destructst_type_closed_ctx in H2. destruct H2 as (Hnst & Hfind & Hctx & Htau & Hwf)...
+    constructor...
+    + constructor; auto. inversion Hnodup... eapply st_type_closed_in_ctx_destruct_oarr_front in Htau...
+    + intros. eapply H3... constructor...
+      (* rewrite state_tystate_same_none... *)
+      (* assert (l_find_right_most Gamma x = None) as Hfindx... *)
+      intros e_x He_xD. assert (exists c0 : constant, e_x -->* c0) as He_xE... apply inv_ctx_implies_head in H1. apply destruct_ctx_inv_one in H1. destruct H1...
+      destruct tau_a.
+      { eapply step_preserve_ctx_denotation... apply eta_drop_lete_not_bot... }
+      { eapply step_preserve_ctx_denotation_over... apply eta_drop_lete_not_bot... }
+Qed.
 
 Lemma ctx_inv_front_destruct_over: forall st a T phi Gamma,
     ctx_inv st ((a, Oty ({{v:T | phi}})) :: Gamma) ->
     (forall (c_x: constant), tmR_aux st ({{v:T | phi}}) c_x -> ctx_inv (a |-> c_x; st) Gamma).
-Admitted.
+Proof with eauto.
+  intros.
+  induction Gamma. inversion H; subst.
+  assert (type_ctx_no_dup (st\_ st _/) ((x, tau):: nil)). constructor...
+  apply type_ctx_no_dup_implies_head_free in H4. apply l_find_right_most_none_neq_hd in H4. exfalso...
+  assert (type_ctx_no_dup (st\_ st _/) ((a, Oty ({{v:T | phi}})) :: nil) ). constructor...
+  apply type_ctx_no_dup_implies_head_free in H1. apply l_find_right_most_none_neq_hd in H1. exfalso...
+Qed.
 
 Global Hint Resolve ctx_inv_front_destruct_over: core.
 
@@ -236,11 +320,19 @@ Lemma ctx_inv_drop_last_weakening: forall st Gamma x xty,
         (forall e, tmR_in_ctx_aux st Gamma tau e -> tmR_in_ctx_aux st ((x, xty)::Gamma) tau e)).
 Proof with eauto.
   intros st Gamma x xty H tau Hwf e HH.
-  eapply tmR_in_ctx_pre_weakening... apply app_one_is_cons.
+  rewrite <- app_one_is_cons.
+  eapply tmR_in_ctx_pre_weakening...
 Qed.
 
 Lemma inv_implies_type_closed_last: forall st Gamma x tau_x,
   ctx_inv st (Gamma ++ ((x, tau_x)::nil)) -> st_type_closed_in_ctx (st\_ st _/) Gamma tau_x.
-Admitted.
+Proof with eauto.
+  intros.
+  inversion H... apply app_one_eq_nil in H2. inversion H2.
+  apply app_inj_tail  in H0. destruct H0. subst...
+  assert (type_ctx_no_dup (st\_ st _/) ((x, tau_x)::nil)). constructor...
+    apply type_ctx_no_dup_implies_head_free in H0. apply l_find_right_most_none_neq_hd in H0. exfalso...
+Qed.
+
 
 Definition well_formed (Gamma: context) (tau: underty) := ctx_inv empty Gamma /\ st_type_closed_in_ctx empty Gamma tau.
